fstar/treedem/MLS.TreeDEM.API.fst
@@ -1,0 +1,181 @@
+module MLS.TreeDEM.API
+
+open Comparse
+open MLS.Crypto
+open MLS.Tree
+open MLS.NetworkTypes
+open MLS.TreeDEM.NetworkTypes
+open MLS.TreeDEM.Keys
+open MLS.TreeDEM.Message.Framing
+open MLS.TreeDEM.API.Types
+open MLS.Result
+
+#set-options "--fuel 0 --ifuel 0"
+
+#push-options "--ifuel 1"
+type treedem_init_arguments (bytes:Type0) {|bytes_like bytes|} = {
+  tree_height: nat;
+  my_leaf_index: leaf_index tree_height 0;
+  group_context: group_context_nt bytes;
+  encryption_secret: bytes;
+  sender_data_secret: bytes;
+  membership_key: bytes;
+  my_signature_key: bytes;
+  verification_keys: tree (option (signature_public_key_nt bytes)) unit tree_height 0;
+}
+#pop-options
+
+val init:
+  #bytes:Type0 -> {|crypto_bytes bytes|} ->
+  treedem_init_arguments bytes ->
+  result (treedem_state bytes)
+let init #bytes #cb {tree_height; my_leaf_index; group_context; encryption_secret; sender_data_secret; membership_key; my_signature_key; verification_keys} =
+  let? leaf_tree_secret = leaf_kdf encryption_secret my_leaf_index in
+  let? my_application_ratchet = init_application_ratchet leaf_tree_secret in
+  let? my_handshake_ratchet = init_handshake_ratchet leaf_tree_secret in
+  return ({
+    tree_height;
+    my_leaf_index; 
+    group_context;
+    encryption_secret;
+    sender_data_secret;
+    membership_key;
+    my_signature_key;
+    my_handshake_ratchet;
+    my_application_ratchet;
+    verification_keys;
+  } <: treedem_state bytes)
+
+val protect_public:
+  #bytes:Type0 -> {|crypto_bytes bytes|} ->
+  treedem_state bytes ->
+  msg:authenticated_content_nt bytes{msg.wire_format == WF_mls_public_message} ->
+  result (public_message_nt bytes)
+let protect_public #bytes #cb st msg =
+  authenticated_content_to_public_message msg (mk_static_option st.group_context) (mk_static_option st.membership_key)
+
+val unprotect_public:
+  #bytes:Type0 -> {|crypto_bytes bytes|} ->
+  treedem_state bytes ->
+  public_message_nt bytes ->
+  result (authenticated_content_nt bytes)
+let unprotect_public #bytes #cb st msg =
+  public_message_to_authenticated_content msg (mk_static_option st.group_context) (mk_static_option st.membership_key)
+
+val protect_private:
+  #bytes:Type0 -> {|crypto_bytes bytes|} ->
+  treedem_state bytes ->
+  msg:authenticated_content_nt bytes{msg.wire_format == WF_mls_private_message} ->
+  lbytes bytes 4 ->
+  result (private_message_nt bytes & treedem_state bytes)
+let protect_private #bytes #cb st msg reuse_guard =
+  let ratchet =
+    match msg.content.content.content_type with
+    | CT_application -> st.my_application_ratchet
+    | _ -> st.my_handshake_ratchet
+  in
+  let? (res, new_ratchet) = authenticated_content_to_private_message msg ratchet reuse_guard st.sender_data_secret in
+  let new_st =
+    match msg.content.content.content_type with
+    | CT_application -> { st with my_application_ratchet = new_ratchet }
+    | _ -> { st with my_handshake_ratchet = new_ratchet }
+  in
+  return (res, new_st)
+
+val unprotect_private:
+  #bytes:Type0 -> {|crypto_bytes bytes|} ->
+  treedem_state bytes ->
+  private_message_nt bytes ->
+  result (authenticated_content_nt bytes & treedem_state bytes)
+let unprotect_private #bytes #cb st msg =
+  let? res = private_message_to_authenticated_content msg st.tree_height st.encryption_secret st.sender_data_secret in
+  return (res, st)
+
+val authenticate_non_commit:
+  #bytes:Type0 -> {|crypto_bytes bytes|} ->
+  treedem_state bytes ->
+  wf:wire_format_nt ->
+  msg:framed_content_nt bytes{msg.content.content_type =!= CT_commit} ->
+  sign_nonce bytes ->
+  result (res:authenticated_content_nt bytes{res.wire_format == wf /\ res.content == msg})
+let authenticate_non_commit #bytes #cb st wf msg nonce =
+  let? signature = compute_message_signature st.my_signature_key nonce wf msg (mk_static_option st.group_context) in
+  return ({
+    wire_format = wf;
+    content = msg;
+    auth = {
+      signature;
+      confirmation_tag = ();
+    }
+  } <: res:authenticated_content_nt bytes{res.wire_format == wf /\ res.content == msg})
+
+type half_authenticated_commit (bytes:Type0) {|bytes_like bytes|} = {
+  wire_format: wire_format_nt;
+  content: content:framed_content_nt bytes{content.content.content_type == CT_commit};
+  signature: mls_bytes bytes;
+}
+
+val start_authenticate_commit:
+  #bytes:Type0 -> {|crypto_bytes bytes|} ->
+  treedem_state bytes ->
+  wf:wire_format_nt ->
+  msg:framed_content_nt bytes{msg.content.content_type == CT_commit} ->
+  sign_nonce bytes ->
+  result (res:half_authenticated_commit bytes{res.wire_format == wf /\ res.content == msg})
+let start_authenticate_commit #bytes #cb st wf msg nonce =
+  let? signature = compute_message_signature st.my_signature_key nonce wf msg (mk_static_option st.group_context) in
+  return ({
+    wire_format = wf;
+    content = msg;
+    signature;
+  } <: res:half_authenticated_commit bytes{res.wire_format == wf /\ res.content == msg})
+
+val finish_authenticate_commit:
+  #bytes:Type0 -> {|crypto_bytes bytes|} ->
+  msg:half_authenticated_commit bytes ->
+  bytes -> bytes ->
+  result (res:authenticated_content_nt bytes{res.wire_format == msg.wire_format /\ res.content == msg.content})
+let finish_authenticate_commit #bytes #cb msg confirmation_key confirmed_transcript_hash  =
+  let? confirmation_tag = compute_message_confirmation_tag confirmation_key confirmed_transcript_hash in
+  let? confirmation_tag = mk_mls_bytes (confirmation_tag <: bytes) "finish_authenticate_commit" "confirmation_tag" in
+  return ({
+    wire_format = msg.wire_format;
+    content = msg.content;
+    auth = {
+      signature = msg.signature;
+      confirmation_tag;
+    }
+  } <: res:authenticated_content_nt bytes{res.wire_format == msg.wire_format /\ res.content == msg.content})
+
+val verify_signature:
+  #bytes:Type0 -> {|crypto_bytes bytes|} ->
+  treedem_state bytes ->
+  authenticated_content_nt bytes ->
+  bool
+let verify_signature #bytes #cb st msg =
+  let opt_verif_key = 
+    match msg.content.sender with
+    | S_member leaf_index -> (
+      if not (leaf_index < pow2 st.tree_height) then None
+      else (
+        leaf_at st.verification_keys leaf_index
+      )
+    )
+    | _ -> None //TODO
+  in
+  match opt_verif_key with
+  | None -> false
+  | Some verif_key ->
+    check_message_signature verif_key msg.auth.signature msg.wire_format msg.content (mk_static_option st.group_context)
+
+val verify_confirmation_tag:
+  #bytes:Type0 -> {|crypto_bytes bytes|} ->
+  treedem_state bytes ->
+  authenticated_content_nt bytes ->
+  bytes -> bytes ->
+  result bool
+let verify_confirmation_tag #bytes #cb st msg confirmation_key confirmed_transcript_hash =
+  match msg.content.content.content_type with
+  | CT_commit ->
+    check_authenticated_content_confirmation_tag msg confirmation_key confirmed_transcript_hash
+  | _ -> internal_failure "verify_confirmation_tag: not a commit"
